messageInvariantPrototypes/twoPhaseCommit/centralized_labels/readme.md
@@ -1,0 +1,3 @@
+# Readme
+
+This version uses labels
